src/library/tactic/reflect_tactic.cpp
@@ -1,0 +1,95 @@
+/*
+Copyright (c) 2015 Daniel Selsam. All rights reserved.
+Released under Apache 2.0 license as described in the file LICENSE.
+Author: Daniel Selsam
+*/
+#include "util/lazy_list_fn.h"
+#include "util/fresh_name.h"
+#include "kernel/type_checker.h"
+#include "kernel/error_msgs.h"
+#include "library/constants.h"
+#include "library/reducible.h"
+#include "library/unifier.h"
+#include "library/app_builder.h"
+#include "library/quoted_expr.h"
+#include "library/tactic/tactic.h"
+#include "library/tactic/elaborate.h"
+#include "library/tactic/expr_to_tactic.h"
+
+namespace lean {
+tactic reflect_goal_tactic(elaborate_fn const & elab, expr const & denote_fn) {
+    return tactic([=](environment const & env, io_state const & ios, proof_state const & s) {
+            proof_state new_s = s;
+            goals const & gs  = new_s.get_goals();
+            if (!gs) {
+                throw_no_goal_if_enabled(s);
+                return proof_state_seq();
+            }
+            expr t            = head(gs).get_type();
+
+            goal const & g      = head(gs);
+            substitution subst  = new_s.get_subst();
+            auto tc             = mk_type_checker(env);
+            constraint_seq cs;
+
+            expr lhs, rhs;
+            if (!is_eq(t, lhs, rhs)) {
+                throw_tactic_exception_if_enabled(new_s, [=](formatter const & fmt) {
+                        format r = format("invalid 'reflect' tactic, the goal type must be an equality");
+                        return r;
+                    });
+                return proof_state_seq();
+            }
+
+            app_builder ab(env, ios.get_options());
+            expr new_lhs = mk_app(denote_fn, mk_quoted_expr(lhs));
+            expr new_rhs = mk_app(denote_fn, mk_quoted_expr(rhs));
+            expr new_t = ab.mk_app(get_eq_name(), new_lhs, new_rhs);
+
+            if (tc->is_def_eq(t, new_t, justification(), cs)) {
+                if (cs) {
+                    unifier_config cfg(ios.get_options());
+                    buffer<constraint> cs_buf;
+                    cs.linearize(cs_buf);
+                    to_buffer(new_s.get_postponed(), cs_buf);
+                    unify_result_seq rseq = unify(env, cs_buf.size(), cs_buf.data(), subst, cfg);
+                    return map2<proof_state>(rseq, [=](pair<substitution, constraints> const & p) -> proof_state {
+                            substitution const & subst    = p.first;
+                            constraints const & postponed = p.second;
+                            substitution new_subst = subst;
+                            expr final_e = new_subst.instantiate_all(new_t);
+                            expr M       = g.mk_meta(mk_fresh_name(), final_e);
+                            goal new_g(M, final_e);
+                            assign(new_subst, g, M);
+                            return proof_state(new_s, cons(new_g, tail(gs)), new_subst, postponed);
+                        });
+                }
+                expr M   = g.mk_meta(mk_fresh_name(), new_t);
+                goal new_g(M, new_t);
+                assign(subst, g, M);
+                return proof_state_seq(proof_state(new_s, cons(new_g, tail(gs)), subst));
+            } else {
+                    throw_tactic_exception_if_enabled(new_s, [=](formatter const & fmt) {
+                            format r = format("invalid 'reflect' tactic, the quoting and denoting yields new goal type");
+                            r += pp_indent_expr(fmt, new_t);
+                            r += compose(line(), format("which does not match the goal type"));
+                            r += pp_indent_expr(fmt, t);
+                            return r;
+                        });
+                    return proof_state_seq();
+
+            }
+            return proof_state_seq();
+        });
+}
+
+void initialize_reflect_tactic() {
+    register_tac(get_tactic_reflect_name(),
+                 [](type_checker &, elaborate_fn const & fn, expr const & e, pos_info_provider const *) {
+                     check_tactic_expr(app_arg(e), "invalid 'reflect' tactic, invalid argument");
+                     return reflect_goal_tactic(fn, get_tactic_expr_expr(app_arg(e)));
+                 });
+}
+void finalize_reflect_tactic() {
+}
+}
