src/library/tactic/reflect_tactic.h
@@ -1,0 +1,12 @@
+/*
+Copyright (c) 2015 Daniel Selsam. All rights reserved.
+Released under Apache 2.0 license as described in the file LICENSE.
+Author: Daniel Selsam
+*/
+#pragma once
+#include "library/tactic/tactic.h"
+
+namespace lean {
+void initialize_reflect_tactic();
+void finalize_reflect_tactic();
+}
