library/data/reflection.lean
@@ -12,10 +12,11 @@ namespace lean
     | imax   : level → level → level
     | param  : name → level
     | global : name → level
-  
+
     inductive expr : Type₁ :=
     | var   : ℕ → expr
     | const : name  → list level → expr
+    | loc   : name  → expr → expr
     | meta  : name  → expr → expr
     | sort  : level → expr
     | pi    : name  → expr → expr → expr
